deps/poulet4/lib/P4cub/Transformations/Lifted.v
@@ -1,0 +1,74 @@
+Require Export Poulet4.P4cub.Syntax.Syntax
+        Poulet4.P4cub.Transformations.Statementize
+        Coq.Numbers.DecimalString
+        Coq.Strings.Ascii Coq.Strings.String.
+Import P4cub.P4cubNotations StringSyntax Field.FieldTactics.
+Module E := P4cub.Expr.
+Module ST := P4cub.Stmt.
+
+Section Lifted.
+  (*Open Scope char_scope.*)
+  Open Scope string_scope.
+  
+  Context {tags_t : Type}.
+  
+  Inductive lifted_expr : E.e tags_t -> Prop :=
+  | lifted_bool b i :
+      lifted_expr <{ BOOL b @ i }>
+  | lifted_var x τ i :
+      lifted_expr <{ Var x:τ @ i }>
+  | lifted_member e x τ i :
+      lifted_expr e ->
+      lifted_expr <{ Mem e:τ dot x @ i }>
+  | lifted_error err i :
+      lifted_expr <{ Error err @ i }>
+  | lifted_matchkind mk i :
+      lifted_expr <{ Matchkind mk @ i }>
+  | lifted_access e z i :
+      lifted_expr e ->
+      lifted_expr <{ Access e[z] @ i }>.
+
+  Local Hint Constructors lifted_expr : core.
+
+  Ltac transformExpr_destr :=
+    match goal with
+    | |- context [TransformExpr _ ?e ?env]
+      => destruct (TransformExpr _ e env) as [[? ?] ?] eqn:?; simpl in *
+    end.
+
+  Ltac transformExpr_destr_hyp :=
+    match goal with
+    | H: context [TransformExpr _ ?e ?env] |- _
+      => destruct (TransformExpr _ e env) as [[? ?] ?] eqn:?; simpl in *
+    end.
+
+  Ltac fold_destr :=
+    match goal with
+    | |- context [fold_left ?f ?l ?acc]
+      => destruct (fold_left f l acc) as [[? ?] ?] eqn:Hfoldl; simpl in *
+    | |- context [fold_right ?f ?acc ?l]
+      => destruct (fold_right f acc l) as [[? ?] ?] eqn:Hfoldl; simpl in *
+    end.
+  
+  (*Arguments VarNameGen.new_var env : simpl never.*)
+  
+  Lemma TransformExpr_lifted : forall e env,
+      lifted_expr (snd (fst (TransformExpr _ e env))).
+  Proof.
+    intro e; induction e using custom_e_ind;
+      intro env; unravel in *;
+        repeat transformExpr_destr; auto;
+        try (generalize dependent env;
+             unfold TransformExprList';
+             ind_list_Forall; intro env; simpl;
+             try fold_destr; auto; assumption);
+        try (generalize dependent env;
+             unfold TransformFields', Field.fold;
+             ind_list_predfs; intro env; simpl; auto;
+             try fold_destr; auto;
+             destruct p as [? ?] eqn:Heqp;
+             repeat transformExpr_destr; auto; assumption);
+        try (constructor; specialize IHe with env;
+             transformExpr_destr_hyp; inv Heqp; auto; assumption).
+  Qed.
+End Lifted.
