deps/poulet4/lib/P4cub/Transformations/StatementizeCorrect.v
@@ -1,0 +1,32 @@
+Set Warnings "-custom-entry-overridden".
+Require Export Poulet4.P4cub.Syntax.Syntax
+        Poulet4.P4cub.Transformations.Statementize.
+Require Export Poulet4.P4cub.BigStep.BigStep
+        Poulet4.P4cub.Envn.
+Import P4cub.P4cubNotations
+       Env.EnvNotations
+       Val.ValueNotations
+       Step.
+Module E := P4cub.Expr.
+Module ST := P4cub.Stmt.
+
+Section Correct.
+  Context {tags_t : Type}.
+
+  (* Type Soundness for statements
+     would be useful for this.
+     Knowing [exists] an environment for
+     the statement to evaluate to
+     (worry about this later). *)
+  Lemma expr_semantic_pres : forall (e e' : E.e tags_t) env env' s,
+      TransformExpr _ e env = (s, e', env') ->
+      forall ϵ v pkt fe ctx, (* ctx & fe shouldn't matter. *)
+        ⟨ ϵ, e ⟩ ⇓ v ->
+        exists ϵ',
+          ⟪ pkt , fe , ϵ , ctx , s ⟫ ⤋ ⟪ ϵ' , C , pkt ⟫ /\
+          (* packet [pkt] shouldn't change in stmt evalution. *)
+          ⟨ ϵ', e' ⟩ ⇓ v (*/\ ϵ ⊆ ϵ' (define sub-env relation) *).
+  Proof.
+    (* TODO. *)
+  Abort.
+End Correct.
